feat(data/list/sigma,alist): basic functions on association lists

data/list/basic.lean
@@ -1650,86 +1650,41 @@ end
 
 end find
 
-section lookup
-variables [decidable_eq α] {σ : α → Type v}
+/- lookmap -/
+section lookmap
+variables (f : α → option α)
 
-/-- `lookup a l` is the first value in `l` corresponding to the key `a`,
-  or `none` if no such element exists. -/
-def lookup (a : α) : list (sigma σ) → option (σ a)
-| []             := none
-| (⟨a', b⟩ :: l) := if h : a' = a then some (eq.rec_on h b) else lookup l
+/-- `lookmap` is a combination of `lookup` and `filter_map`.
+  `lookmap f l` will apply `f : α → option α` to each element of the list,
+  replacing `a -> b` at the first value `a` in the list such that `f a = some b`. -/
+def lookmap (f : α → option α) : list α → list α
+| []     := []
+| (a::l) :=
+  match f a with
+  | some b := b :: l
+  | none   := a :: lookmap l
+  end
 
-@[simp] theorem lookup_nil (a : α) : lookup a [] = @none (σ a) := rfl
+@[simp] theorem lookmap_nil : [].lookmap f = [] := rfl
 
-@[simp] theorem lookup_cons_eq (l) (a : α) (b : σ a) : lookup a (⟨a, b⟩::l) = some b :=
-dif_pos rfl
+theorem lookmap_cons_none {a : α} (l : list α) (h : f a = none) :
+  (a :: l).lookmap f = a :: l.lookmap f :=
+by simp [lookmap, h]
 
-@[simp] theorem lookup_cons_ne (l) {a} :
-  ∀ s : sigma σ, a ≠ s.1 → lookup a (s::l) = lookup a l
-| ⟨a', b⟩ h := dif_neg h.symm
+theorem lookmap_cons_some {a b : α} (l : list α) (h : f a = some b) :
+  (a :: l).lookmap f = b :: l :=
+by simp [lookmap, h]
 
-theorem lookup_eq_none {a : α} : ∀ {l : list (sigma σ)},
-  lookup a l = none ↔ ∀ b : σ a, sigma.mk a b ∉ l
-| []             := by simp
-| (⟨a', b⟩ :: l) := begin
-  by_cases h : a = a',
-  { subst a', simp, exact λ H, H b (or.inl rfl) },
-  { simp [h, lookup_eq_none] },
+theorem lookmap_map_eq {g : α → β} (h : ∀ a (b ∈ f a), g a = g b) :
+  ∀ l : list α, map g (l.lookmap f) = map g l
+| []     := rfl
+| (a::l) := begin
+  cases h' : f a with b,
+  { simp [lookmap_cons_none _ _ h', lookmap_map_eq] },
+  { simp [lookmap_cons_some _ _ h', h _ _ h'] }
 end
 
-theorem of_mem_lookup
-  {a : α} {b : σ a} : ∀ {l : list (sigma σ)}, b ∈ lookup a l → sigma.mk a b ∈ l
-| (⟨a', b'⟩ :: l) H := begin
-  by_cases h : a = a',
-  { subst a', simp at H, simp [H] },
-  { simp [h] at H, exact or.inr (of_mem_lookup H) }
-end
-
-theorem map_lookup_eq_find (a : α) : ∀ l : list (sigma σ),
-  (lookup a l).map (sigma.mk a) = find (λ s, a = s.1) l
-| [] := rfl
-| (⟨a', b'⟩ :: l) := begin
-  by_cases h : a = a',
-  { subst a', simp },
-  { simp [h, map_lookup_eq_find] }
-end
-
-/-- `lookup_all a l` is the first value in `l` corresponding to the key `a`,
-  or `none` if no such element exists. -/
-def lookup_all (a : α) : list (sigma σ) → list (σ a)
-| []             := []
-| (⟨a', b⟩ :: l) := if h : a' = a then eq.rec_on h b :: lookup_all l else lookup_all l
-
-@[simp] theorem lookup_all_nil (a : α) : lookup_all a [] = @nil (σ a) := rfl
-
-@[simp] theorem lookup_all_cons_eq (l) (a : α) (b : σ a) :
-  lookup_all a (⟨a, b⟩::l) = b :: lookup_all a l :=
-dif_pos rfl
-
-@[simp] theorem lookup_all_cons_ne (l) {a} :
-  ∀ s : sigma σ, a ≠ s.1 → lookup_all a (s::l) = lookup_all a l
-| ⟨a', b⟩ h := dif_neg h.symm
-
-theorem lookup_all_eq_nil {a : α} : ∀ {l : list (sigma σ)},
-  lookup_all a l = [] ↔ ∀ b : σ a, sigma.mk a b ∉ l
-| []             := by simp
-| (⟨a', b⟩ :: l) := begin
-  by_cases h : a = a',
-  { subst a', simp, exact λ H, H b (or.inl rfl) },
-  { simp [h, lookup_all_eq_nil] },
-end
-
-theorem head_lookup_all (a : α) : ∀ l : list (sigma σ),
-  head' (lookup_all a l) = lookup a l
-| []             := by simp
-| (⟨a', b⟩ :: l) := by by_cases h : a = a'; [{subst h, simp}, simp *]
-
-theorem mem_lookup_all {a : α} {b : σ a} :
-  ∀ {l : list (sigma σ)}, b ∈ lookup_all a l ↔ sigma.mk a b ∈ l
-| []              := by simp
-| (⟨a', b'⟩ :: l) := by by_cases h : a = a'; [{subst h, simp *}, simp *]
-
-end lookup
+end lookmap
 
 /-- `indexes_of a l` is the list of all indexes of `a` in `l`.
   `indexes_of a [a, b, a, a] = [0, 2, 3]` -/
@@ -4039,27 +3994,6 @@ by rw [sublists'_eq_sublists, nodup_map_iff reverse_injective,
 
 end nodup
 
-section ndkeys
-variables {σ : α → Type v}
-
-def ndkeys (l : list (sigma σ)) : Prop :=
-(l.map sigma.fst).nodup
-
-variables [decidable_eq α]
-
-theorem mem_lookup_iff {a : α} {b : σ a} {l : list (sigma σ)} (nd : l.ndkeys) :
-  b ∈ lookup a l ↔ sigma.mk a b ∈ l :=
-⟨of_mem_lookup, λ h, begin
-  induction l with s l IH generalizing b; cases h with h h,
-  { subst s, simp },
-  { cases s with a' b',
-    by_cases h' : a = a',
-    { subst h', simp,
-      exact (not_mem_of_nodup_cons nd).elim (mem_map_of_mem sigma.fst h : _) },
-    { simpa [h'] using IH (nodup_of_nodup_cons nd) h } }
-end⟩
-
-end ndkeys
 /- erase duplicates function -/
 
 section erase_dup
