data/list/alist.lean
@@ -1,0 +1,32 @@
+import data.list.sigma
+
+universes u v w
+
+structure alist {α : Type u} (β : α → Type v) : Type (max u v) :=
+(val : list (sigma β))
+(nd : val.knodup)
+
+namespace alist
+variables {α : Type u} {β : α → Type v}
+
+instance : has_mem α (alist β) := ⟨λ a s, ∃ b : β a, sigma.mk a b ∈ s.val⟩
+
+variables [decidable_eq α]
+
+def lookup (a : α) (s : alist β) : option (β a) :=
+s.val.lookup a
+
+theorem lookup_is_some {a : α} {s : alist β} :
+  (s.lookup a).is_some ↔ a ∈ s := list.lookup_is_some
+
+instance (a : α) (s : alist β) : decidable (a ∈ s) :=
+decidable_of_iff _ lookup_is_some
+
+def replace (a : α) (b : β a) (s : alist β) : alist β :=
+⟨list.kreplace a b s.val, (list.kreplace_knodup a b).2 s.nd⟩
+
+/-- Fold a function over the key-value pairs in the map -/
+def foldl {δ : Type w} (f : δ → Π a, β a → δ) (d : δ) (m : alist β) : δ :=
+m.val.foldl (λ r a, f r a.1 a.2) d
+
+end alist
